Directory tree example

functional-programming-lean/scripts/build-examples.py
@@ -1,0 +1,15 @@
+import json
+import subprocess
+import sys
+
+
+def main():
+    if len(sys.argv) > 1:
+        if sys.argv[1] == "supports":
+            sys.exit(0)
+    subprocess.run('lake build', shell=True, cwd=f'../examples', check=True, capture_output=True)
+    context, book_contents = json.load(sys.stdin)
+    print(json.dumps(book_contents))
+
+if __name__ == '__main__':
+    main()
