examples/Examples/MonadTransformers.lean
@@ -1,4 +1,5 @@
 import Examples.Support
+import Examples.Monads
 
 namespace Evaluator
 
@@ -70,43 +71,119 @@ def evaluate : Expr → Eval Int
 end Evaluator
 
 
-
-
 namespace DirTree
 
-structure Config where
-  useAscii : Bool := false
-  currentPrefix := ""
 
-def preFile := "├──"
-def preDir := "│  "
+book declaration {{{ Config }}}
+  structure Config where
+    useASCII : Bool := false
+    currentPrefix : String := ""
+stop book declaration
+
+
+book declaration {{{ filenames }}}
+  def Config.preFile (cfg : Config) :=
+    if cfg.useASCII then "|--" else "├──"
+
+  def Config.preDir (cfg : Config) :=
+    if cfg.useASCII then "|  " else "│  "
+
+  def Config.fileName (cfg : Config) (file : String) : String :=
+    s!"{cfg.currentPrefix}{cfg.preFile} {file}"
+
+  def Config.dirName (cfg : Config) (dir : String) : String :=
+    s!"{cfg.currentPrefix}{cfg.preFile} {dir}/"
+stop book declaration
+
+
+book declaration {{{ inDirectory }}}
+  def Config.inDirectory (cfg : Config) : Config :=
+    {cfg with currentPrefix := cfg.preDir ++ " " ++ cfg.currentPrefix}
+stop book declaration
+
+book declaration {{{ configFromArgs }}}
+  def configFromArgs : List String → Option Config
+    | [] => some {}
+    | ["--ascii"] => some {useASCII := true}
+    | _ => none
+stop book declaration
+
+
+book declaration {{{ usage }}}
+def usage : String :=
+  "Usage: doug [--ascii]
+Options:
+\t--ascii\tUse ASCII characters to display the directory structure"
+stop book declaration
+
+
+book declaration {{{ Entry }}}
+  inductive Entry where
+    | file : String → Entry
+    | dir : String → Entry
+stop book declaration
+
+
+book declaration {{{ toEntry }}}
+  def toEntry (path : System.FilePath) : IO (Option Entry) := do
+    match path.components.getLast? with
+    | none => pure (some (.dir ""))
+    | some "." | some ".." => pure none
+    | some name =>
+      pure (some (if (← path.isDir) then .dir name else .file name))
+stop book declaration
 
 namespace Old
-def showFile (cfg : Config) (file : String) : IO Unit := do
-  IO.println s!"{cfg.currentPrefix} {file}"
 
-def showDirName (cfg : Config) (dir : String) : IO Unit := do
-  IO.println s!"{cfg.currentPrefix} {dir}/"
 
-def doList : (List α) → (α → IO Unit) → IO Unit
-  | [], _ => pure ()
-  | x :: xs, action => do
-    action x
-    doList xs action
+book declaration {{{ OldShowFile }}}
+  def showFileName (cfg : Config) (file : String) : IO Unit := do
+    IO.println (cfg.fileName file)
 
-partial def dirTree (cfg : Config) (path : System.FilePath) : IO Unit := do
-  match path.fileName with
-  | none => pure ()
-  | some name =>
-    if !(← path.isDir) then
-      showFile cfg name
-    else
+  def showDirName (cfg : Config) (dir : String) : IO Unit := do
+    IO.println (cfg.dirName dir)
+stop book declaration
+
+
+book declaration {{{ doList }}}
+  def doList : (List α) → (α → IO Unit) → IO Unit
+    | [], _ => pure ()
+    | x :: xs, action => do
+      action x
+      doList xs action
+stop book declaration
+
+book declaration {{{ OldDirTree }}}
+  partial def dirTree (cfg : Config) (path : System.FilePath) : IO Unit := do
+    match (← toEntry path) with
+    | none => pure ()
+    | some (.file name) => showFileName cfg name
+    | some (.dir name) =>
       showDirName cfg name
       let contents ← path.readDir
-      let newConfig := {cfg with currentPrefix := preDir ++ " " ++ cfg.currentPrefix}
-      doList contents.toList (fun d =>
-        dirTree newConfig d.path)
+      let newConfig := cfg.inDirectory
+      doList contents.toList fun d =>
+        dirTree newConfig d.path
+stop book declaration
+
+book declaration {{{ OldMain }}}
+  def main (args : List String) : IO UInt32 := do
+    match configFromArgs args with
+    | some config =>
+      dirTree config (← IO.currentDir)
+      pure 0
+    | none =>
+      IO.eprintln s!"Didn't understand argument(s) {" ".separate args}\n"
+      IO.eprintln usage
+      pure 1
+stop book declaration
+
+-- #eval main ["--ascii"]
+
+
 end Old
+
+namespace Readerish
 
 def ConfigIO (β : Type) (α : Type) : Type := β → IO α
 
@@ -124,13 +201,11 @@ def locally (change : β → γ) (action : ConfigIO γ α) : ConfigIO β α :=
 def io (action : IO α) : ConfigIO β α :=
   fun _ => action
 
-def showFile (file : String) : ConfigIO Config Unit := do
-  let cfg ← config
-  io (IO.println s!"{cfg.currentPrefix} {file}")
+def showFileName (file : String) : ConfigIO Config Unit := do
+  io (IO.println ((← config).fileName file))
 
 def showDirName (dir : String) : ConfigIO Config Unit := do
-  let cfg ← config
-  io (IO.println s!"{cfg.currentPrefix} {dir}/")
+  io (IO.println ((← config).dirName dir))
 
 def doList : (List α) → (α → ConfigIO β Unit) → ConfigIO β Unit
   | [], _ => pure ()
@@ -139,17 +214,53 @@ def doList : (List α) → (α → ConfigIO β Unit) → ConfigIO β Unit
     doList xs action
 
 def inDir (cfg : Config) : Config :=
-  {cfg with currentPrefix := preDir ++ " " ++ cfg.currentPrefix}
+  {cfg with currentPrefix := cfg.preDir ++ " " ++ cfg.currentPrefix}
 
-partial def dirTree' (path : System.FilePath) : ConfigIO Config Unit := do
+partial def dirTree (path : System.FilePath) : ConfigIO Config Unit := do
   match path.fileName with
   | none => pure ()
   | some name =>
     if !(← io path.isDir) then
-      showFile name
+      showFileName name
     else
       showDirName name
       let contents ← io path.readDir
-      locally inDir (doList contents.toList (fun d => dirTree' d.path))
+      locally inDir (doList contents.toList (fun d => dirTree d.path))
+end Readerish
+
+namespace T
+
+abbrev ConfigIO (β : Type) (α : Type) : Type := ReaderT β IO α
+
+def showFileName (file : String) : ConfigIO Config Unit := do
+  IO.println s!"{(← read).currentPrefix} {file}"
+
+def showDirName (dir : String) : ConfigIO Config Unit := do
+  IO.println s!"{(← read).currentPrefix} {dir}/"
+
+def inDir (cfg : Config) : Config :=
+  {cfg with currentPrefix := cfg.preDir ++ " " ++ cfg.currentPrefix}
+
+partial def dirTree (path : System.FilePath) : ConfigIO Config Unit := do
+  match path.fileName with
+  | none => pure ()
+  | some name =>
+    if !(← path.isDir) then
+      showFileName name
+    else
+      showDirName name
+      for d in (← path.readDir) do dirTree d.path
+
+end T
 
 end DirTree
+
+
+namespace MyVersions
+
+def ReaderT (ρ : Type) (m : Type → Type) (α : Type) : Type :=
+  ρ → m α
+
+end MyVersions
+
+example : ReaderT = MyVersions.ReaderT := by rfl
