examples/Examples/Doug1.lean
@@ -1,0 +1,3 @@
+import Examples.MonadTransformers
+
+def main := DirTree.Old.main
