examples/Examples/Monads/Conveniences.lean
@@ -41,3 +41,106 @@ book declaration {{{ mirrorNew }}}
     | .branch l x r => .branch (mirror r) x (mirror l)
 stop book declaration
 end New
+
+
+book declaration {{{ Weekday }}}
+  inductive Weekday where
+    | monday
+    | tuesday
+    | wednesday
+    | thursday
+    | friday
+    | saturday
+    | sunday
+    deriving Repr
+stop book declaration
+
+namespace A
+
+book declaration {{{ isWeekendA }}}
+  def Weekday.isWeekend (day : Weekday) : Bool :=
+    match day with
+    | Weekday.saturday => true
+    | Weekday.sunday => true
+    | _ => false
+stop book declaration
+end A
+
+namespace B
+book declaration {{{ isWeekendB }}}
+  def Weekday.isWeekend (day : Weekday) : Bool :=
+    match day with
+    | .saturday => true
+    | .sunday => true
+    | _ => false
+stop book declaration
+end B
+
+namespace C
+book declaration {{{ isWeekendC }}}
+  def Weekday.isWeekend (day : Weekday) : Bool :=
+    match day with
+    | .saturday | .sunday => true
+    | _ => false
+stop book declaration
+end C
+
+namespace D
+book declaration {{{ isWeekendD }}}
+  def Weekday.isWeekend : Weekday → Bool
+    | .saturday | .sunday => true
+    | _ => false
+stop book declaration
+end D
+
+
+
+book declaration {{{ condense }}}
+  def condense : α ⊕ α → α
+    | .inl x | .inr x => x
+stop book declaration
+
+
+book declaration {{{ stringy }}}
+  def stringy : Nat ⊕ Weekday → String
+    | .inl x | .inr x => s!"It is {repr x}"
+stop book declaration
+
+#eval stringy (.inl 5)
+#eval stringy (.inr .monday)
+
+
+book declaration {{{ getTheNat }}}
+  def getTheNat : (Nat × α) ⊕ (Nat × β) → Nat
+    | .inl (n, x) | .inr (n, y) => n
+stop book declaration
+
+
+
+expect error {{{ getTheAlpha }}}
+  def getTheAlpha : (Nat × α) ⊕ (Nat × α) → α
+    | .inl (n, x) | .inr (n, y) => x
+message
+"unknown identifier 'x'"
+end expect
+
+book declaration {{{ getTheString }}}
+  def str := "Some string"
+
+  def getTheString : (Nat × String) ⊕ (Nat × β) → String
+    | .inl (n, str) | .inr (n, y) => str
+stop book declaration
+
+
+expect info {{{ getOne }}}
+  #eval getTheString (.inl (20, "twenty") : (Nat × String) ⊕ (Nat × String))
+message
+"\"twenty\""
+end expect
+
+
+expect info {{{ getTwo }}}
+  #eval getTheString (.inr (20, "twenty"))
+message
+"\"Some string\""
+end expect
