functional-programming-lean/src/monad-transformers/reader-io.md
@@ -1,0 +1,116 @@
+# Combining IO and Reader
+
+One case where a reader monad can be useful is when there is some notion of the "current configuration" of the application that is passed through many recursive calls.
+An example of such a program is `tree`, which recursively prints the files in the current directory and its subdirectories, indicating their tree structure using characters.
+The version of `tree` in this chapter, called `doug` after the mighty Douglas Fir tree that adorns the west coast of North America, provides the option of Unicode box-drawing characters or their ASCII equivalents when indicating directory structure.
+
+For example, the following commands create a directory structure and some empty files in a directory called `doug-demo`:
+```
+$ cd doug-demo
+$ {{#command {doug-demo} {doug} {mkdir -p a/b/c} }}
+$ {{#command {doug-demo} {doug} {mkdir -p a/d} }}
+$ {{#command {doug-demo} {doug} {mkdir -p a/e/f} }}
+$ {{#command {doug-demo} {doug} {touch a/b/hello} }}
+$ {{#command {doug-demo} {doug} {touch a/d/another-file} }}
+$ {{#command {doug-demo} {doug} {touch a/e/still-another-file-again} }}
+```
+Running `doug` results in the following:
+```
+$ {{#command {doug-demo} {doug} {doug} }}
+{{#command_out {doug} {doug} }}
+```
+
+## Implementation
+
+Internally, `doug` passes a configuration value downwards as it recursively traverses the directory structure.
+This configuration contains two fields: `useASCII` determines whether to use Unicode box-drawing characters or ASCII vertical line and dash characters to indicate structure, and `currentPrefix` contains a string to prepend to each line of output.
+As the current directory deepens, the prefix string accumulates indicators of being in a directory.
+The configuration is a structure:
+```lean
+{{#example_decl Examples/MonadTransformers.lean Config}}
+```
+Type classes are really structures behind the scenes, and structures can have default field definitions in just the same way that type classes can have default method definitions.
+In this case, `Config` defaults to Unicode display with no prefix.
+
+Users who invoke `doug` will need to be able to provide command-line arguments.
+The usage information is as follows:
+```lean
+{{#example_decl Examples/MonadTransformers.lean usage}}
+```
+Accordingly, a configuration can be constructed by examining a list of command-line arguments:
+```lean
+{{#example_decl Examples/MonadTransformers.lean configFromArgs}}
+```
+
+The `main` function is a wrapper around an inner worker, called `dirTree`, that shows the contents of a directory using a configuration.
+Before calling `dirTree`, `main` is responsible for processing command-line arguments.
+It must also return the appropriate exit code to the operating system:
+```lean
+{{#example_decl Examples/MonadTransformers.lean OldMain}}
+```
+
+Not all paths should be shown in the directory tree.
+In particular, files named `.` or `..` should be skipped, as they are actually features used for navigation rather than files _per se_.
+Of those files that should be shown, there are two kinds: ordinary files and directories:
+```lean
+{{#example_decl Examples/MonadTransformers.lean Entry}}
+```
+To determine whether a file should be shown, along with which kind of entry it is, `doug` uses `toEntry`:
+```lean
+{{#example_decl Examples/MonadTransformers.lean toEntry}}
+```
+`System.FilePath.components` converts a path into a list of path components, splitting the name at directory separators.
+If there is no last component, then the path is the root directory.
+If the last component is a special navigation file (`.` or `..`), then the file should be excluded.
+Otherwise, directories and files are wrapped in the corresponding constructors.
+
+Lean's logic has no way to know that directory trees are finite.
+Indeed, some systems allow the construction of circular directory structures.
+Thus, `dirTree` is declared `partial`:
+```lean
+{{#example_decl Examples/MonadTransformers.lean OldDirTree}}
+```
+When the filename doesn't correspond to an entry in the tree (e.g. because it is `..`), `dirTree` does nothing.
+When the filename is an ordinary file, `dirTree` calls a helper to show it with the current configuration.
+When the filename is a directory, it is shown with a helper, and then its contents are recursively shown in a new configuration in which the prefix has been extended to account for being in a new directory.
+
+Showing the names of files and directories is achieved with `showFileName` and `showDirName`:
+```lean
+{{#example_decl Examples/MonadTransformers.lean OldShowFile}}
+```
+Both of these helpers delegate to functions on `Config` that take the ASCII vs Unicode setting into account:
+```lean
+{{#example_decl Examples/MonadTransformers.lean filenames}}
+```
+Similarly, `Config.inDirectory` extends the prefix with a directory marker:
+```lean
+{{#example_decl Examples/MonadTransformers.lean inDirectory}}
+```
+
+Iterating an IO action over a list of directory contents is achieved using `doList`:
+```lean
+{{#example_decl Examples/MonadTransformers.lean doList}}
+```
+
+## Using a Custom Monad
+
+
+
+
+## Exercises
+
+### Controlling the Display of Dotfiles
+
+Files whose names being with a dot character (`'.'`) typically represent files that should usually be hidden, such as source-control metadata and configuration files.
+Modify `doug` with an option to show or hide filenames that begin with a dot.
+This option should be controlled with a `-a` command-line option.
+
+### Starting Directory as Argument
+
+Modify `doug` so that it takes a starting directory as an additional command-line argument.
+
+### Support 
+
+### Monadic Error Handling
+
+Right now, errors such as invalid 
